Disable tail calls in variadic functions
Variadic functions can use the stack frame to store values of registers.
Hence, a pointer within the stack frame can be put in a va_list, and
the stack frame should not be deallocated before a function call that
may use this va_list.

Fixes: #473

backend/Tailcall.v
@@ -93,6 +93,7 @@ Definition transf_instr (f: function) (pc: node) (instr: instruction) :=
 
 Definition transf_function (f: function) : function :=
   if zeq f.(fn_stacksize) 0
+  && option_eq zeq f.(fn_sig).(sig_cc).(cc_vararg) None
   then RTL.transf_function (transf_instr f) f
   else f.
 
